\section{Getting $\alpha$}

\begin{align*}
2-\alpha &= \frac{4}{3} + \frac{4}{3} \alpha + \varepsilon + \varepsilon \alpha\\
\frac{6}{3} - \frac{3}{3}\alpha &= \frac{4}{3} + \frac{4}{3} \alpha +
\frac{3}{3}\varepsilon + \frac{3}{3}\varepsilon \alpha\\
\frac{6}{3} - \frac{4}{3} - \frac{3}{3}\varepsilon &= \frac{4}{3} \alpha +
\frac{3}{3}\alpha + \frac{3}{3}\varepsilon \alpha\\
\frac{2}{3} - \frac{3}{3}\varepsilon &= \frac{7}{3} \alpha + \frac{3}{3}\varepsilon \alpha\\
2 - 3 \varepsilon &= ( 7 + 3 \varepsilon) \alpha\\
\frac{2-3\varepsilon}{7+3\varepsilon} &= \alpha\\
\alpha &= \frac{2}{7} - \varepsilon'
\end{align*}

